Fix bug in local simulation's tailcall case: now returned state should be related.

backend/RTLSim.v
@@ -91,7 +91,15 @@ Inductive _state_lsim
     (Hargs: list_forall2 (mrelT_ops.(sem_value) mrel) args2_src args2_tgt)
     (mrel2:mrelT) (Hmrel2: mrelT_ops.(sem) mrel2 mem2_src mem2_tgt)
     (Hmrel2_le: mrelT_ops.(le) mrel mrel2)
-    (Hmrel2_le_public: mrelT_ops.(le_public) mrel_entry mrel2)
+    (Hreturn:
+       forall mrel3 st3_src st3_tgt mem3_src mem3_tgt vres_src vres_tgt
+              (Hvres: mrelT_ops.(sem_value) mrel3 vres_src vres_tgt)
+              (Hst3_src: st3_src = Returnstate stack2_src vres_src mem3_src)
+              (Hst3_tgt: st3_tgt = Returnstate stack2_tgt vres_tgt mem3_tgt)
+              (Hmrel3_le: mrelT_ops.(le_public) mrel2 mrel3)
+              (Hst3_mem: mrelT_ops.(sem) mrel3 mem3_src mem3_tgt),
+       exists i3,
+         state_lsim mrel3 i3 st3_src st3_tgt)
 
 | _state_lsim_step
     (Hpreserve:
@@ -114,6 +122,9 @@ Lemma state_lsim_mon: monotone4 _state_lsim.
 Proof.
   repeat intro; destruct IN; eauto.
   - eapply _state_lsim_call; eauto.
+    intros. exploit Hreturn; eauto.
+    intros [i3 Hsim]. exists i3. auto.
+  - eapply _state_lsim_tailcall; eauto.
     intros. exploit Hreturn; eauto.
     intros [i3 Hsim]. exists i3. auto.
   - eapply _state_lsim_step; eauto.
